template-coq/theories/monad_utils.v
@@ -244,3 +244,4 @@ Section MonadAllAll.
     sq. constructor; assumption.
   Defined.
 End MonadAllAll.
+
